src/ocaml-output/FStar_Syntax_Const.ml
@@ -220,6 +220,8 @@ let fstar_tactics_lid: Prims.string -> FStar_Ident.lident =
     FStar_Ident.lid_of_path (FStar_List.append ["FStar"; "Tactics"] [s])
       FStar_Range.dummyRange
 let tactic_lid: FStar_Ident.lident = fstar_tactics_lid "tactic"
+let u_tac_lid: FStar_Ident.lident = fstar_tactics_lid "__tac"
+let tac_effect_lid: FStar_Ident.lident = fstar_tactics_lid "TAC"
 let by_tactic_lid: FStar_Ident.lident = fstar_tactics_lid "by_tactic"
 let reify_tactic_lid: FStar_Ident.lident = fstar_tactics_lid "reify_tactic"
 let quote_lid: FStar_Ident.lident =
