ulib/FStar.Tactics.Types.fsti
@@ -1,6 +1,6 @@
 module FStar.Tactics.Types
 
-type binder //FStar.Syntax.Syntax.binder
-type term
-type env
-type fv
+assume new type binder //FStar.Syntax.Syntax.binder
+assume new type term
+assume new type env
+assume new type fv
